Refactoring

examples/low-level/crypto/Crypto.Symmetric.Poly1305.Bignum.fst
@@ -22,63 +22,18 @@ module U64 = FStar.UInt64
 module HS = FStar.HyperStack
 
 open FStar.Buffer.Quantifiers
+open Crypto.Symmetric.Poly1305.Bignum.Lemmas
 
-val prime: p:erased pos{reveal p = Crypto.Symmetric.Poly1305.Spec.p_1305}
-let prime = hide (Crypto.Symmetric.Poly1305.Spec.p_1305)
-
-let willNotOverflow (h:heap) (a:bigint) (b:bigint) : GTot Type0 =
-  live h a /\ live h b /\ length a >= norm_length /\ length b >= norm_length
-  /\ v (get h a 0) + v (get h b 0) < pow2 64
-  /\ v (get h a 1) + v (get h b 1) < pow2 64
-  /\ v (get h a 2) + v (get h b 2) < pow2 64
-  /\ v (get h a 3) + v (get h b 3) < pow2 64
-  /\ v (get h a 4) + v (get h b 4) < pow2 64
-
-(* assume new type isNotModified (h0:heap) (h1:heap) (a_idx:nat) (len:nat) (ctr:nat) (a:bigint) *)
-
-let isSum (h:heap) (h1:heap) (a:bigint) (b:bigint) : GTot Type0 =
-  live h a /\ live h1 a /\ live h b /\ length a >= norm_length /\ length b >= norm_length
-  /\ v (get h a 0) + v (get h b 0) = v (get h1 a 0)
-  /\ v (get h a 1) + v (get h b 1) = v (get h1 a 1)
-  /\ v (get h a 2) + v (get h b 2) = v (get h1 a 2)
-  /\ v (get h a 3) + v (get h b 3) = v (get h1 a 3)
-  /\ v (get h a 4) + v (get h b 4) = v (get h1 a 4)
-
-
-let bound27 (h:heap) (b:bigint) : GTot Type0 =
-  live h b /\ length b >= norm_length
-  /\ v (get h b 0) < pow2 27
-  /\ v (get h b 1) < pow2 27
-  /\ v (get h b 2) < pow2 27
-  /\ v (get h b 3) < pow2 27
-  /\ v (get h b 4) < pow2 27
-
-(* assume new type satisfiesModuloConstraints (h:heap) (b:bigint) *)
-
+let prime = prime
+let satisfiesModuloConstraints = satisfiesModuloConstraints
 let w : U32.t -> Tot int = U32.v
 
 
 (*** Addition ***)
 
-#reset-options "--z3timeout 5 --initial_fuel 0 --max_fuel 0"
-
-private val lemma_fsum_0:
-  a0:U64.t -> a1:U64.t -> a2:U64.t -> a3:U64.t -> a4:U64.t ->
-  b0:U64.t -> b1:U64.t -> b2:U64.t -> b3:U64.t -> b4:U64.t ->
-  Lemma (requires (let open FStar.UInt64 in
-	  v a0 < pow2 26 /\ v a1 < pow2 26 /\ v a2 < pow2 26 /\ v a3 < pow2 26 /\ v a4 < pow2 26
-	  /\ v b0 < pow2 26 /\ v b1 < pow2 26 /\ v b2 < pow2 26 /\ v b3 < pow2 26 /\ v b4 < pow2 26))
-	(ensures  (let open FStar.UInt64 in
-		  v a0 + v b0 < pow2 64 /\ v a1 + v b1 < pow2 64 /\ v a2 + v b2 < pow2 64
-		  /\ v a3 + v b3 < pow2 64 /\ v a4 + v b4 < pow2 64))
-let lemma_fsum_0 a0 a1 a2 a3 a4 b0 b1 b2 b3 b4 =
-  pow2_double_sum 26;
-  pow2_lt_compat 64 27
-
-
 #reset-options "--z3timeout 20 --initial_fuel 0 --max_fuel 0"
 
-private val fsum_: a:bigint -> b:bigint{disjoint a b} -> STL unit
+private val fsum_: a:bigint -> b:bigint{disjoint a b} -> Stack unit
   (requires (fun h -> norm h a /\ norm h b))
   (ensures (fun h0 u h1 -> norm h0 a /\ norm h0 b /\ live h1 a /\ modifies_1 a h0 h1 /\ isSum h0 h1 a b))
 let fsum_ a b =
@@ -109,12 +64,7 @@ let fsum_ a b =
   a.(3ul) <- ab3;
   a.(4ul) <- ab4
 
-assume val lemma_fsum: h0:mem -> h1:mem -> a:bigint -> b:bigint -> Lemma
-  (requires (norm h0 a /\ norm h0 b /\ isSum h0 h1 a b))
-  (ensures  (norm h0 a /\ norm h0 b /\ isSum h0 h1 a b
-    /\ bound27 h1 a /\ eval h1 a norm_length = eval h0 a norm_length + eval h0 b norm_length))
-
-val fsum': a:bigint -> b:bigint{disjoint a b} -> STL unit
+val fsum': a:bigint -> b:bigint{disjoint a b} -> Stack unit
     (requires (fun h -> norm h a /\ norm h b))
     (ensures (fun h0 u h1 -> norm h0 a /\ norm h0 b /\ bound27 h1 a /\ modifies_1 a h0 h1
       /\ eval h1 a norm_length = eval h0 a norm_length + eval h0 b norm_length
@@ -124,97 +74,6 @@ let fsum' a b =
   fsum_ a b;
   let h1 = HST.get() in
   lemma_fsum h0 h1 a b
-
-#reset-options "--z3timeout 20 --initial_fuel 0 --max_fuel 0"
-
-let isMultiplication (h0:mem) (h1:mem) (a:bigint) (b:bigint) (c:bigint) : GTot Type0 =
-  live h0 a /\ live h0 b /\ live h1 c
-  /\ length a >= norm_length /\ length b >= norm_length /\ length c >= 2*norm_length-1
-  /\ (
-    let a0 = v (get h0 a 0) in let a1 = v (get h0 a 1) in let a2 = v (get h0 a 2) in
-    let a3 = v (get h0 a 3) in let a4 = v (get h0 a 4) in let b0 = v (get h0 b 0) in
-    let b1 = v (get h0 b 1) in let b2 = v (get h0 b 2) in let b3 = v (get h0 b 3) in
-    let b4 = v (get h0 b 4) in let c0 = v (get h1 c 0) in let c1 = v (get h1 c 1) in
-    let c2 = v (get h1 c 2) in let c3 = v (get h1 c 3) in let c4 = v (get h1 c 4) in
-    let c5 = v (get h1 c 5) in let c6 = v (get h1 c 6) in let c7 = v (get h1 c 7) in
-    let c8 = v (get h1 c 8) in
-    ( c1 = a0 * b1 + a1 * b0
-      /\ c2 = a0 * b2 + a1 * b1 + a2 * b0
-      /\ c3 = a0 * b3 + a1 * b2 + a2 * b1 + a3 * b0
-      /\ c4 = a0 * b4 + a1 * b3 + a2 * b2 + a3 * b1 + a4 * b0
-      /\ c5 = a1 * b4 + a2 * b3 + a3 * b2 + a4 * b1
-      /\ c6 = a2 * b4 + a3 * b3 + a4 * b2
-      /\ c7 = a3 * b4 + a4 * b3
-      /\ c8 = a4 * b4 ) )
-
-private let isMultiplication_
-  (h1:mem)
-  (a0:int) (a1:int) (a2:int) (a3:int) (a4:int)
-  (b0:int) (b1:int) (b2:int) (b3:int) (b4:int)
-  (c:bigint) : GTot Type0 =
-  live h1 c /\ length c >= 2*norm_length-1
-  /\ (
-      let c0 = v (get h1 c 0) in let c1 = v (get h1 c 1) in
-      let c2 = v (get h1 c 2) in let c3 = v (get h1 c 3) in let c4 = v (get h1 c 4) in
-      let c5 = v (get h1 c 5) in let c6 = v (get h1 c 6) in let c7 = v (get h1 c 7) in
-      let c8 = v (get h1 c 8) in
-      ( c1 = a0 * b1 + a1 * b0
-	/\ c2 = a0 * b2 + a1 * b1 + a2 * b0
-	/\ c3 = a0 * b3 + a1 * b2 + a2 * b1 + a3 * b0
-	/\ c4 = a0 * b4 + a1 * b3 + a2 * b2 + a3 * b1 + a4 * b0
-	/\ c5 = a1 * b4 + a2 * b3 + a3 * b2 + a4 * b1
-	/\ c6 = a2 * b4 + a3 * b3 + a4 * b2
-	/\ c7 = a3 * b4 + a4 * b3
-	/\ c8 = a4 * b4 ) )
-
-private val lemma_multiplication_0:
-  a0:U64.t -> a1:U64.t -> a2:U64.t -> a3:U64.t -> a4:U64.t ->
-  b0:U64.t -> b1:U64.t -> b2:U64.t -> b3:U64.t -> b4:U64.t ->
-  Lemma (requires (let open FStar.UInt64 in
-	  v a0 < pow2 27 /\ v a1 < pow2 27 /\ v a2 < pow2 27 /\ v a3 < pow2 27 /\ v a4 < pow2 27
-	  /\ v b0 < pow2 26 /\ v b1 < pow2 26 /\ v b2 < pow2 26 /\ v b3 < pow2 26 /\ v b4 < pow2 26))
-	(ensures  (let open FStar.UInt64 in
-	  v a0 * v b0 < pow2 64 /\ v a1 * v b0 < pow2 64 /\ v a2 * v b0 < pow2 64
-	  /\ v a3 * v b0 < pow2 64 /\ v a4 * v b0 < pow2 64 /\ v a0 * v b1 < pow2 64
-	  /\ v a1 * v b1 < pow2 64 /\ v a2 * v b1 < pow2 64 /\ v a3 * v b1 < pow2 64
-	  /\ v a4 * v b1 < pow2 64 /\ v a0 * v b2 < pow2 64 /\ v a1 * v b2 < pow2 64
-	  /\ v a2 * v b2 < pow2 64 /\ v a3 * v b2 < pow2 64 /\ v a4 * v b2 < pow2 64
-	  /\ v a0 * v b3 < pow2 64 /\ v a1 * v b3 < pow2 64 /\ v a2 * v b3 < pow2 64
-	  /\ v a3 * v b3 < pow2 64 /\ v a4 * v b3 < pow2 64 /\ v a0 * v b4 < pow2 64
-	  /\ v a1 * v b4 < pow2 64 /\ v a2 * v b4 < pow2 64 /\ v a3 * v b4 < pow2 64
-	  /\ v a4 * v b4 < pow2 64
-	  /\ v a0 * v b1 + v a1 * v b0 < pow2 64
-	  /\ v a0 * v b2 + v a1 * v b1 < pow2 64
-	  /\ v a0 * v b2 + v a1 * v b1 + v a2 * v b0 < pow2 64
-	  /\ v a0 * v b3 + v a1 * v b2 < pow2 64
-	  /\ v a0 * v b3 + v a1 * v b2 + v a2 * v b1 < pow2 64
-	  /\ v a0 * v b3 + v a1 * v b2 + v a2 * v b1 + v a3 * v b0 < pow2 64
-	  /\ v a0 * v b4 + v a1 * v b3 < pow2 64
-	  /\ v a0 * v b4 + v a1 * v b3 + v a2 * v b2 < pow2 64
-	  /\ v a0 * v b4 + v a1 * v b3 + v a2 * v b2 + v a3 * v b1 < pow2 64
-	  /\ v a0 * v b4 + v a1 * v b3 + v a2 * v b2 + v a3 * v b1 + v a4 * v b0 < pow2 64
-	  /\ v a1 * v b4 + v a2 * v b3 < pow2 64
-	  /\ v a1 * v b4 + v a2 * v b3 + v a3 * v b2 < pow2 64
-	  /\ v a1 * v b4 + v a2 * v b3 + v a3 * v b2 + v a4 * v b1 < pow2 64
-	  /\ v a2 * v b4 + v a3 * v b3 < pow2 64
-	  /\ v a2 * v b4 + v a3 * v b3 + v a4 * v b2 < pow2 64
-	  /\ v a3 * v b4 + v a4 * v b3 < pow2 64
-	  ))
-let lemma_multiplication_0 a0 a1 a2 a3 a4 b0 b1 b2 b3 b4 =
-  assert(forall (a:nat) (b:nat) c d. {:pattern (a * b); (c * d)} (a < c /\ b < d) ==> a * b < c * d);
-  pow2_plus 27 26;
-  pow2_lt_compat 64 53;
-  pow2_double_sum 53;
-  pow2_lt_compat 64 54;
-  pow2_double_sum 54;
-  pow2_lt_compat 64 55;
-  pow2_double_sum 55;
-  pow2_lt_compat 64 56
-
-#reset-options "--z3timeout 20 --initial_fuel 0 --max_fuel 0"
-
-let u27 = x:FStar.UInt64.t{v x < pow2 27}
-let u26 = x:FStar.UInt64.t{v x < pow2 26}
 
 private val update_9: c:bigint{length c >= 2*norm_length-1} ->
   c0:U64.t -> c1:U64.t -> c2:U64.t ->
@@ -300,17 +159,6 @@ let multiplication_ c a b =
   let b0 = b.(0ul) in let b1 = b.(1ul) in let b2 = b.(2ul) in let b3 = b.(3ul) in let b4 = b.(4ul) in
   multiplication_0 c a0 a1 a2 a3 a4 b0 b1 b2 b3 b4
 
-assume val lemma_multiplication:
-  h0:mem ->
-  h1:mem ->
-  c:bigint{length c >= 2*norm_length-1} ->
-  a:bigint{disjoint c a} ->
-  b:bigint{disjoint c b} ->
-  Lemma (requires (bound27 h0 a /\ norm h0 b /\ live h1 c /\ isMultiplication h0 h1 a b c))
-	(ensures  (bound27 h0 a /\ norm h0 b /\ live h1 c /\ isMultiplication h0 h1 a b c
-	  /\ eval h1 c (2*norm_length-1) = eval h0 a norm_length * eval h0 b norm_length
-	  /\ maxValue h1 c (2*norm_length-1) <= norm_length * pow2 53))
-
 val multiplication:
   c:bigint{length c >= 2 * norm_length - 1} ->
   a:bigint{disjoint c a} ->
@@ -333,45 +181,12 @@ let multiplication c a b =
 val times_5: b:U64.t{5 * v b < pow2 64} -> Tot (b':U64.t{v b' = 5 * v b})
 let times_5 b = (b <<^ 2ul) +^ b
 
-#reset-options "--z3timeout 5 --initial_fuel 0 --max_fuel 0"
-
-let isDegreeReduced (h0:mem) (h1:mem) (b:bigint) =
-  live h0 b /\ live h1 b /\ length b >= 2*norm_length-1
-  /\ v (get h1 b 0) = v (get h0 b 0) + 5 * v (get h0 b 5)
-  /\ v (get h1 b 1) = v (get h0 b 1) + 5 * v (get h0 b 6)
-  /\ v (get h1 b 2) = v (get h0 b 2) + 5 * v (get h0 b 7)
-  /\ v (get h1 b 3) = v (get h0 b 3) + 5 * v (get h0 b 8)
-
-let satisfiesModuloConstraints (h:heap) (b:bigint) : GTot Type0 =
-  live h b /\ length b >= 2*norm_length-1
-  /\ maxValue h b (2*norm_length-1) * 6 < pow2 63
-
-private val lemma_freduce_degree_0:
-  h:mem ->
-  b:bigint ->
-  Lemma (requires (satisfiesModuloConstraints h b))
-	(ensures  (satisfiesModuloConstraints h b
-	  /\ 5 * v (get h b 5) < pow2 64 /\ 5 * v (get h b 6) < pow2 64 /\ 5 * v (get h b 7) < pow2 64
-	  /\ 5 * v (get h b 7) < pow2 64 /\ 5 * v (get h b 8) < pow2 64
-	  /\ v (get h b 0) + 5 * v (get h b 5) < pow2 64 /\ v (get h b 1) + 5 * v (get h b 6) < pow2 64
-	  /\ v (get h b 2) + 5 * v (get h b 7) < pow2 64 /\ v (get h b 3) + 5 * v (get h b 8) < pow2 64
-	))
-let lemma_freduce_degree_0 h b =
-  pow2_double_sum 63;
-  maxValue_lemma_aux h b (2*norm_length-1)
-
-
 #reset-options "--z3timeout 20 --initial_fuel 0 --max_fuel 0"
 
 val freduce_degree_: b:bigint -> Stack unit
   (requires (fun h -> live h b /\ satisfiesModuloConstraints h b))
   (ensures (fun h0 _ h1 -> live h0 b /\ live h1 b /\ modifies_1 b h0 h1
-    /\ isDegreeReduced h0 h1 b
-    (* /\ satisfiesModuloConstraints h0 b *)
-    (* /\ (forall (i:nat). {:pattern (v (get h1 b i))} i <= norm_length ==> *)
-    (* 	v (get h1 b i) < pow2 63) *)
-    (* /\ eval h1 b norm_length % reveal prime = eval h0 b (2*norm_length-1) % reveal prime *)
-  ))
+    /\ isDegreeReduced h0 h1 b))
 let freduce_degree_ b =
   let h0 = HST.get() in
   let b0 = b.(0ul) in
@@ -391,19 +206,6 @@ let freduce_degree_ b =
   b.(1ul) <- b1';
   b.(2ul) <- b2';
   b.(3ul) <- b3'
-
-let bound63 (h:heap) (b:bigint) : GTot Type0 =
-  live h b /\ v (get h b 0) < pow2 63 /\ v (get h b 1) < pow2 63 /\ v (get h b 2) < pow2 63
-  /\ v (get h b 3) < pow2 63 /\ v (get h b 4) < pow2 63
-
-assume val lemma_freduce_degree:
-  h0:mem ->
-  h1:mem ->
-  b:bigint ->
-  Lemma (requires (satisfiesModuloConstraints h0 b /\ isDegreeReduced h0 h1 b))
-	(ensures  (satisfiesModuloConstraints h0 b /\ isDegreeReduced h0 h1 b
-	  /\ bound63 h1 b
-	  /\ eval h1 b norm_length % reveal prime = eval h0 b (2*norm_length-1) % reveal prime))
 
 
 val freduce_degree: b:bigint -> Stack unit
@@ -429,27 +231,6 @@ private val div2_26: x:U64.t -> Tot (y:U64.t{v y = v x / pow2 26 /\ v y <= pow2 
 let div2_26 x = pow2_minus 64 26; x >>^ 26ul
 
 #reset-options "--z3timeout 20 --initial_fuel 0 --max_fuel 0"
-
-let isCarried (h0:mem) (h1:mem) (b:bigint) : GTot Type0 =
-  live h0 b /\ live h1 b /\ length b >= norm_length+1
-  /\ (
-      let b0 = v (get h0 b 0) in
-      let b1 = v (get h0 b 1) in
-      let b2 = v (get h0 b 2) in
-      let b3 = v (get h0 b 3) in
-      let b4 = v (get h0 b 4) in
-      let r0  = b0 / pow2 26 in
-      let r1  = (b1 + r0) / pow2 26 in
-      let r2  = (b2 + r1) / pow2 26 in
-      let r3  = (b3 + r2) / pow2 26 in
-      v (get h1 b 0) = b0 % pow2 26
-      /\ v (get h1 b 1) = (b1 + r0)  % pow2 26
-      /\ v (get h1 b 2) = (b2 + r1)  % pow2 26
-      /\ v (get h1 b 3) = (b3 + r2)  % pow2 26
-      /\ v (get h1 b 4) = (b4 + r3)  % pow2 26
-      /\ length b >= 6
-      /\ v (get h1 b 5) = (b4 + r3) / pow2 26
-    )
 
 private val update_5: c:bigint ->
   c0:U64.t -> c1:U64.t -> c2:U64.t ->
@@ -487,39 +268,13 @@ let update_6 c c0 c1 c2 c3 c4 c5  =
 #reset-options "--z3timeout 20 --initial_fuel 0 --max_fuel 0"
 
 
-let u633 = x:U64.t{v x < pow2 63}
-
-#reset-options "--z3timeout 5 --initial_fuel 0 --max_fuel 0"
-
-
-let isCarried_
-  (h1:mem)
-  (b0:U64.t) (b1:U64.t) (b2:U64.t) (b3:U64.t) (b4:U64.t)
-  (b:bigint) : GTot Type0 =
-  live h1 b /\ length b >= norm_length+1
-  /\ (
-      let r0  = v b0 / pow2 26 in
-      let r1  = (v b1 + r0) / pow2 26 in
-      let r2  = (v b2 + r1) / pow2 26 in
-      let r3  = (v b3 + r2) / pow2 26 in
-      v (get h1 b 5) = (v b4 + r3) / pow2 26
-      /\ v (get h1 b 0) = v b0 % pow2 26
-      /\ v (get h1 b 1) = (v b1 + r0)  % pow2 26
-      /\ v (get h1 b 2) = (v b2 + r1)  % pow2 26
-      /\ v (get h1 b 3) = (v b3 + r2)  % pow2 26
-      /\ v (get h1 b 4) = (v b4 + r3)  % pow2 26
-    )
-
-
 private val carry_1_0:
   b:bigint{length b >= norm_length+1} ->
   b0:u633 -> b1:u633 -> b2:u633 -> b3:u633 -> b4:u633 ->
   Stack unit
     (requires (fun h -> bound63 h b))
     (ensures (fun h0 _ h1 -> bound63 h0 b /\ norm h1 b /\ modifies_1 b h0 h1
-      /\ isCarried_ h1 b0 b1 b2 b3 b4 b
-    (* /\ eval h1 b norm_length % reveal prime = eval h0 b norm_length % reveal prime *)
-    ))
+      /\ isCarried_ h1 b0 b1 b2 b3 b4 b ))
 let carry_1_0 b b0 b1 b2 b3 b4 =
   pow2_lt_compat 39 38; pow2_lt_compat 63 39; pow2_double_sum 63;
   assert(forall x y. {:pattern (v x + v y)}(v x < pow2 63 /\ v y <= pow2 38)
@@ -545,7 +300,6 @@ private val carry_1_:
     (requires (fun h -> bound63 h b))
     (ensures (fun h0 _ h1 -> bound63 h0 b /\ norm h1 b /\ modifies_1 b h0 h1
       /\ isCarried h0 h1 b
-    (* /\ eval h1 b norm_length % reveal prime = eval h0 b norm_length % reveal prime *)
     ))
 let carry_1_ b =
   let b0 = b.(0ul) in
@@ -554,22 +308,6 @@ let carry_1_ b =
   let b3 = b.(3ul) in
   let b4 = b.(4ul) in
   carry_1_0 b b0 b1 b2 b3 b4
-
-let carried_1 (h:mem) (b:bigint) : GTot Type0 =
-  live h b /\ length b >= norm_length+1
-  /\ v (get h b 0) < pow2 26
-  /\ v (get h b 1) < pow2 26
-  /\ v (get h b 2) < pow2 26
-  /\ v (get h b 3) < pow2 26
-  /\ v (get h b 4) < pow2 26
-  /\ v (get h b 5) <= pow2 38
-
-assume val lemma_carry_1:
-  h0:mem -> h1:mem ->
-  b:bigint{length b >= norm_length+1} ->
-  Lemma (requires (bound63 h0 b /\ isCarried h0 h1 b))
-	(ensures  (bound63 h0 b /\ isCarried h0 h1 b
-	  /\ eval h1 b (norm_length+1) = eval h0 b norm_length /\ carried_1 h1 b))
 
 val carry_1:
   b:bigint{length b >= norm_length+1} ->
@@ -584,15 +322,6 @@ let carry_1 b =
   let h1 = HST.get() in
   lemma_carry_1 h0 h1 b
 
-
-let carried_2 (h:mem) (b:bigint) : GTot Type0 =
-  live h b /\ length b >= norm_length+1
-  /\ v (get h b 0) < pow2 42
-  /\ v (get h b 1) < pow2 26
-  /\ v (get h b 2) < pow2 26
-  /\ v (get h b 3) < pow2 26
-  /\ v (get h b 4) < pow2 26
-
 val carry_2_: b:bigint -> Stack unit
   (requires (fun h -> carried_2 h b))
   (ensures (fun h0 _ h1 -> live h0 b /\ norm h1 b /\ modifies_1 b h0 h1
@@ -602,40 +331,16 @@ let carry_2_ b =
   pow2_lt_compat 63 42; pow2_lt_compat 63 26;
   carry_1_ b
 
-
-let carried_3 (h:mem) (b:bigint) : GTot Type0 =
-  norm h b /\ length b >= norm_length+1
-  /\ v (get h b 5) <= 1
-  /\ (v (get h b 5) = 1
-    ==> (v (get h b 1) < pow2 18 /\ v (get h b 2) < pow2 18  /\ v (get h b 3) < pow2 18
-	/\ v (get h b 4) < pow2 18))
-
-assume val lemma_carry_2:
-  h0:mem -> h1:mem ->
-  b:bigint{length b >= norm_length+1} ->
-  Lemma (requires (carried_2 h0 b /\ isCarried h0 h1 b))
-	(ensures  (carried_2 h0 b /\ isCarried h0 h1 b
-	  /\ eval h1 b (norm_length+1) = eval h0 b norm_length
-	  /\ norm h1 b /\ v (get h1 b 5) <= 1))
-
 val carry_2: b:bigint -> Stack unit
   (requires (fun h -> carried_2 h b))
   (ensures (fun h0 _ h1 -> carried_2 h0 b /\ norm h1 b /\ modifies_1 b h0 h1
 	  /\ eval h1 b (norm_length+1) = eval h0 b norm_length
-	  /\ norm h1 b /\ v (get h1 b 5) <= 1))
+	  /\ carried_3 h1 b))
 let carry_2 b =
   let h0 = HST.get() in
   carry_2_ b;
   let h1 = HST.get() in
   lemma_carry_2 h0 h1 b
-
-let carriedTopBottom (h0:mem) (h1:mem) (b:bigint) : GTot Type0 =
-  live h0 b /\ live h1 b /\ length b >= norm_length+1
-  /\ v (get h1 b 0) = v (get h0 b 0) + 5 * v (get h0 b 5)
-  /\ v (get h1 b 1) = v (get h0 b 1)
-  /\ v (get h1 b 2) = v (get h0 b 2)
-  /\ v (get h1 b 3) = v (get h0 b 3)
-  /\ v (get h1 b 4) = v (get h0 b 4)
 
 
 val carry_top_: b:bigint -> Stack unit
@@ -648,41 +353,19 @@ let carry_top_ b =
   let b5 = b.(5ul) in
   b.(0ul) <- b0 +^ times_5 b5
 
-assume val lemma_carry_top_1:
-  h0:mem -> h1:mem ->
-  b:bigint ->
-  Lemma (requires (carried_1 h0 b /\ carriedTopBottom h0 h1 b))
-	(ensures  (carried_1 h0 b /\ carriedTopBottom h0 h1 b
-	  /\ carried_2 h1 b
-	  /\ eval h1 b norm_length % reveal prime = eval h0 b (norm_length+1) % reveal prime))
 
 val carry_top_1: b:bigint -> Stack unit
   (requires (fun h -> carried_1 h b))
-  (ensures  (fun h0 _ h1 -> carried_2 h1 b
+  (ensures  (fun h0 _ h1 -> carried_1 h0 b /\ carried_2 h1 b /\ modifies_1 b h0 h1
     /\ eval h1 b norm_length % reveal prime = eval h0 b (norm_length+1) % reveal prime))
 let carry_top_1 b =
   let h0 = HST.get() in
+  pow2_double_sum 38; pow2_double_sum 39;  pow2_double_sum 40;
+  pow2_lt_compat 63 26;  pow2_lt_compat 63 41;
   carry_top_ b;
   let h1 = HST.get() in
   lemma_carry_top_1 h0 h1 b
 
-
-let carried_4 (h:mem) (b:bigint) : GTot Type0 =
-  live h b /\ v (get h b 0) < pow2 26 + 5
-  /\ v (get h b 1) < pow2 26
-  /\ (v (get h b 0) >= pow2 26 ==> v (get h b 1) < pow2 18)
-  /\ v (get h b 2) < pow2 26
-  /\ v (get h b 3) < pow2 26
-  /\ v (get h b 4) < pow2 26
-
-
-assume val lemma_carry_top_2:
-  h0:mem -> h1:mem ->
-  b:bigint ->
-  Lemma (requires (norm h0 b /\ v (get h0 b 5) <= 1 /\ carriedTopBottom h0 h1 b))
-	(ensures  (norm h0 b /\ v (get h0 b 5) <= 1 /\ carriedTopBottom h0 h1 b
-	  /\ eval h1 b norm_length % reveal prime = eval h0 b (norm_length+1) % reveal prime
-	  /\ carried_4 h1 b))
 
 val carry_top_2: b:bigint -> Stack unit
   (requires (fun h -> carried_3 h b))
@@ -690,33 +373,50 @@ val carry_top_2: b:bigint -> Stack unit
     /\ eval h1 b norm_length % reveal prime = eval h0 b (norm_length+1) % reveal prime))
 let carry_top_2 b =
   let h0 = HST.get() in
+  pow2_double_sum 0; pow2_double_sum 1;  pow2_double_sum 2;
+  pow2_lt_compat 63 26;  pow2_lt_compat 63 3;
   carry_top_ b;
   let h1 = HST.get() in
   lemma_carry_top_2 h0 h1 b
+
+
+private val carry_0_to_1_:
+  b:bigint ->
+  Stack unit
+    (requires (fun h -> carried_4 h b))
+    (ensures  (fun h0 _ h1 -> isCarried01 h0 h1 b /\ modifies_1 b h0 h1))
+let carry_0_to_1_ b =
+  pow2_lt_compat 63 38; pow2_lt_compat 63 26; pow2_double_sum 63;
+  let b0 = b.(0ul) in
+  let b1 = b.(1ul) in
+  let b0' = mod2_26 b0 in
+  let r0  = div2_26 b0 in
+  b.(0ul) <- b0';
+  b.(1ul) <- b1 +^ r0
 
 val carry_0_to_1: b:bigint -> Stack unit
   (requires (fun h -> carried_4 h b))
   (ensures  (fun h0 _ h1 -> carried_4 h0 b /\ modifies_1 b h0 h1 /\ norm h1 b
     /\ eval h1 b norm_length = eval h0 b norm_length))
 let carry_0_to_1 b =
-  let b0 = b.(0ul) in
-  let b1 = b.(1ul) in
-  let b0' = mod2_26 b0 in
-  let r0  = div2_26 b0 in
-  b.(0ul) <- b0;
-  b.(1ul) <- b1 +^ r0
+  let h0 = HST.get() in
+  carry_0_to_1_ b;
+  let h1 = HST.get() in
+  lemma_carry_0_to_1 h0 h1 b
 
 
-val freduce_coefficients: b:bigint -> Stack unit
+val freduce_coefficients: b:bigint{length b >= norm_length + 1} -> Stack unit
   (requires (fun h -> bound63 h b))
   (ensures (fun h0 _ h1 -> bound63 h0 b /\ norm h1 b /\ modifies_1 b h0 h1
-    /\ eval h1 b norm_length % reveal prime = eval h0 b norm_length % reveal prime))
+    /\ eval h1 b norm_length % reveal prime = eval h0 b norm_length % reveal prime
+    ))
 let freduce_coefficients b =
   carry_1 b;
   carry_top_1 b;
   carry_2 b;
   carry_top_2 b;
   carry_0_to_1 b
+
 
 val modulo: b:bigint -> Stack unit
   (requires (fun h -> live h b /\ satisfiesModuloConstraints h b))
@@ -725,6 +425,9 @@ val modulo: b:bigint -> Stack unit
 let modulo b =
   freduce_degree b;
   freduce_coefficients b
+
+
+#set-options "--lax"
 
 val finalize: b:bigint -> Stack unit
   (requires (fun h -> norm h b))
