examples/low-level/crypto/Crypto.Symmetric.Poly1305.Bignum.Lemmas.fst
@@ -1,0 +1,361 @@
+module Crypto.Symmetric.Poly1305.Bignum.Lemmas
+
+open FStar.Mul
+open FStar.Ghost
+(** Machine integers *)
+open FStar.UInt64
+(** Effects and memory layout *)
+open FStar.HyperStack
+open FStar.HST
+(** Buffers *)
+open FStar.Buffer
+(** Mathematical definitions *)
+open Math.Axioms
+open Math.Lib
+open Math.Lemmas
+
+open Crypto.Symmetric.Poly1305.Parameters
+open Crypto.Symmetric.Poly1305.Bigint
+
+module U32 = FStar.UInt32
+module U64 = FStar.UInt64
+module HS = FStar.HyperStack
+
+val prime: p:erased pos{reveal p = Crypto.Symmetric.Poly1305.Spec.p_1305}
+let prime = hide (Crypto.Symmetric.Poly1305.Spec.p_1305)
+
+let willNotOverflow (h:heap) (a:bigint) (b:bigint) : GTot Type0 =
+  live h a /\ live h b /\ length a >= norm_length /\ length b >= norm_length
+  /\ v (get h a 0) + v (get h b 0) < pow2 64
+  /\ v (get h a 1) + v (get h b 1) < pow2 64
+  /\ v (get h a 2) + v (get h b 2) < pow2 64
+  /\ v (get h a 3) + v (get h b 3) < pow2 64
+  /\ v (get h a 4) + v (get h b 4) < pow2 64
+
+let isSum (h:heap) (h1:heap) (a:bigint) (b:bigint) : GTot Type0 =
+  live h a /\ live h1 a /\ live h b /\ length a >= norm_length /\ length b >= norm_length
+  /\ v (get h a 0) + v (get h b 0) = v (get h1 a 0)
+  /\ v (get h a 1) + v (get h b 1) = v (get h1 a 1)
+  /\ v (get h a 2) + v (get h b 2) = v (get h1 a 2)
+  /\ v (get h a 3) + v (get h b 3) = v (get h1 a 3)
+  /\ v (get h a 4) + v (get h b 4) = v (get h1 a 4)
+
+let bound27 (h:heap) (b:bigint) : GTot Type0 =
+  live h b /\ length b >= norm_length
+  /\ v (get h b 0) < pow2 27
+  /\ v (get h b 1) < pow2 27
+  /\ v (get h b 2) < pow2 27
+  /\ v (get h b 3) < pow2 27
+  /\ v (get h b 4) < pow2 27
+
+let w : U32.t -> Tot int = U32.v
+
+
+(*** Addition ***)
+
+#reset-options "--z3timeout 5 --initial_fuel 0 --max_fuel 0"
+
+val lemma_fsum_0:
+  a0:U64.t -> a1:U64.t -> a2:U64.t -> a3:U64.t -> a4:U64.t ->
+  b0:U64.t -> b1:U64.t -> b2:U64.t -> b3:U64.t -> b4:U64.t ->
+  Lemma (requires (let open FStar.UInt64 in
+	  v a0 < pow2 26 /\ v a1 < pow2 26 /\ v a2 < pow2 26 /\ v a3 < pow2 26 /\ v a4 < pow2 26
+	  /\ v b0 < pow2 26 /\ v b1 < pow2 26 /\ v b2 < pow2 26 /\ v b3 < pow2 26 /\ v b4 < pow2 26))
+	(ensures  (let open FStar.UInt64 in
+		  v a0 + v b0 < pow2 64 /\ v a1 + v b1 < pow2 64 /\ v a2 + v b2 < pow2 64
+		  /\ v a3 + v b3 < pow2 64 /\ v a4 + v b4 < pow2 64))
+let lemma_fsum_0 a0 a1 a2 a3 a4 b0 b1 b2 b3 b4 =
+  pow2_double_sum 26;
+  pow2_lt_compat 64 27
+
+
+assume val lemma_fsum: h0:mem -> h1:mem -> a:bigint -> b:bigint -> Lemma
+  (requires (norm h0 a /\ norm h0 b /\ isSum h0 h1 a b))
+  (ensures  (norm h0 a /\ norm h0 b /\ isSum h0 h1 a b
+    /\ bound27 h1 a /\ eval h1 a norm_length = eval h0 a norm_length + eval h0 b norm_length))
+
+#reset-options "--z3timeout 20 --initial_fuel 0 --max_fuel 0"
+
+let isMultiplication (h0:mem) (h1:mem) (a:bigint) (b:bigint) (c:bigint) : GTot Type0 =
+  live h0 a /\ live h0 b /\ live h1 c
+  /\ length a >= norm_length /\ length b >= norm_length /\ length c >= 2*norm_length-1
+  /\ (
+    let a0 = v (get h0 a 0) in let a1 = v (get h0 a 1) in let a2 = v (get h0 a 2) in
+    let a3 = v (get h0 a 3) in let a4 = v (get h0 a 4) in let b0 = v (get h0 b 0) in
+    let b1 = v (get h0 b 1) in let b2 = v (get h0 b 2) in let b3 = v (get h0 b 3) in
+    let b4 = v (get h0 b 4) in let c0 = v (get h1 c 0) in let c1 = v (get h1 c 1) in
+    let c2 = v (get h1 c 2) in let c3 = v (get h1 c 3) in let c4 = v (get h1 c 4) in
+    let c5 = v (get h1 c 5) in let c6 = v (get h1 c 6) in let c7 = v (get h1 c 7) in
+    let c8 = v (get h1 c 8) in
+    ( c1 = a0 * b1 + a1 * b0
+      /\ c2 = a0 * b2 + a1 * b1 + a2 * b0
+      /\ c3 = a0 * b3 + a1 * b2 + a2 * b1 + a3 * b0
+      /\ c4 = a0 * b4 + a1 * b3 + a2 * b2 + a3 * b1 + a4 * b0
+      /\ c5 = a1 * b4 + a2 * b3 + a3 * b2 + a4 * b1
+      /\ c6 = a2 * b4 + a3 * b3 + a4 * b2
+      /\ c7 = a3 * b4 + a4 * b3
+      /\ c8 = a4 * b4 ) )
+
+let isMultiplication_
+  (h1:mem)
+  (a0:int) (a1:int) (a2:int) (a3:int) (a4:int)
+  (b0:int) (b1:int) (b2:int) (b3:int) (b4:int)
+  (c:bigint) : GTot Type0 =
+  live h1 c /\ length c >= 2*norm_length-1
+  /\ (
+      let c0 = v (get h1 c 0) in let c1 = v (get h1 c 1) in
+      let c2 = v (get h1 c 2) in let c3 = v (get h1 c 3) in let c4 = v (get h1 c 4) in
+      let c5 = v (get h1 c 5) in let c6 = v (get h1 c 6) in let c7 = v (get h1 c 7) in
+      let c8 = v (get h1 c 8) in
+      ( c1 = a0 * b1 + a1 * b0
+	/\ c2 = a0 * b2 + a1 * b1 + a2 * b0
+	/\ c3 = a0 * b3 + a1 * b2 + a2 * b1 + a3 * b0
+	/\ c4 = a0 * b4 + a1 * b3 + a2 * b2 + a3 * b1 + a4 * b0
+	/\ c5 = a1 * b4 + a2 * b3 + a3 * b2 + a4 * b1
+	/\ c6 = a2 * b4 + a3 * b3 + a4 * b2
+	/\ c7 = a3 * b4 + a4 * b3
+	/\ c8 = a4 * b4 ) )
+
+val lemma_multiplication_0:
+  a0:U64.t -> a1:U64.t -> a2:U64.t -> a3:U64.t -> a4:U64.t ->
+  b0:U64.t -> b1:U64.t -> b2:U64.t -> b3:U64.t -> b4:U64.t ->
+  Lemma (requires (let open FStar.UInt64 in
+	  v a0 < pow2 27 /\ v a1 < pow2 27 /\ v a2 < pow2 27 /\ v a3 < pow2 27 /\ v a4 < pow2 27
+	  /\ v b0 < pow2 26 /\ v b1 < pow2 26 /\ v b2 < pow2 26 /\ v b3 < pow2 26 /\ v b4 < pow2 26))
+	(ensures  (let open FStar.UInt64 in
+	  v a0 * v b0 < pow2 64 /\ v a1 * v b0 < pow2 64 /\ v a2 * v b0 < pow2 64
+	  /\ v a3 * v b0 < pow2 64 /\ v a4 * v b0 < pow2 64 /\ v a0 * v b1 < pow2 64
+	  /\ v a1 * v b1 < pow2 64 /\ v a2 * v b1 < pow2 64 /\ v a3 * v b1 < pow2 64
+	  /\ v a4 * v b1 < pow2 64 /\ v a0 * v b2 < pow2 64 /\ v a1 * v b2 < pow2 64
+	  /\ v a2 * v b2 < pow2 64 /\ v a3 * v b2 < pow2 64 /\ v a4 * v b2 < pow2 64
+	  /\ v a0 * v b3 < pow2 64 /\ v a1 * v b3 < pow2 64 /\ v a2 * v b3 < pow2 64
+	  /\ v a3 * v b3 < pow2 64 /\ v a4 * v b3 < pow2 64 /\ v a0 * v b4 < pow2 64
+	  /\ v a1 * v b4 < pow2 64 /\ v a2 * v b4 < pow2 64 /\ v a3 * v b4 < pow2 64
+	  /\ v a4 * v b4 < pow2 64
+	  /\ v a0 * v b1 + v a1 * v b0 < pow2 64
+	  /\ v a0 * v b2 + v a1 * v b1 < pow2 64
+	  /\ v a0 * v b2 + v a1 * v b1 + v a2 * v b0 < pow2 64
+	  /\ v a0 * v b3 + v a1 * v b2 < pow2 64
+	  /\ v a0 * v b3 + v a1 * v b2 + v a2 * v b1 < pow2 64
+	  /\ v a0 * v b3 + v a1 * v b2 + v a2 * v b1 + v a3 * v b0 < pow2 64
+	  /\ v a0 * v b4 + v a1 * v b3 < pow2 64
+	  /\ v a0 * v b4 + v a1 * v b3 + v a2 * v b2 < pow2 64
+	  /\ v a0 * v b4 + v a1 * v b3 + v a2 * v b2 + v a3 * v b1 < pow2 64
+	  /\ v a0 * v b4 + v a1 * v b3 + v a2 * v b2 + v a3 * v b1 + v a4 * v b0 < pow2 64
+	  /\ v a1 * v b4 + v a2 * v b3 < pow2 64
+	  /\ v a1 * v b4 + v a2 * v b3 + v a3 * v b2 < pow2 64
+	  /\ v a1 * v b4 + v a2 * v b3 + v a3 * v b2 + v a4 * v b1 < pow2 64
+	  /\ v a2 * v b4 + v a3 * v b3 < pow2 64
+	  /\ v a2 * v b4 + v a3 * v b3 + v a4 * v b2 < pow2 64
+	  /\ v a3 * v b4 + v a4 * v b3 < pow2 64
+	  ))
+let lemma_multiplication_0 a0 a1 a2 a3 a4 b0 b1 b2 b3 b4 =
+  assert(forall (a:nat) (b:nat) c d. {:pattern (a * b); (c * d)} (a < c /\ b < d) ==> a * b < c * d);
+  pow2_plus 27 26;
+  pow2_lt_compat 64 53;
+  pow2_double_sum 53;
+  pow2_lt_compat 64 54;
+  pow2_double_sum 54;
+  pow2_lt_compat 64 55;
+  pow2_double_sum 55;
+  pow2_lt_compat 64 56
+
+#reset-options "--z3timeout 20 --initial_fuel 0 --max_fuel 0"
+
+let u27 = x:FStar.UInt64.t{v x < pow2 27}
+let u26 = x:FStar.UInt64.t{v x < pow2 26}
+
+assume val lemma_multiplication:
+  h0:mem ->
+  h1:mem ->
+  c:bigint{length c >= 2*norm_length-1} ->
+  a:bigint{disjoint c a} ->
+  b:bigint{disjoint c b} ->
+  Lemma (requires (bound27 h0 a /\ norm h0 b /\ live h1 c /\ isMultiplication h0 h1 a b c))
+	(ensures  (bound27 h0 a /\ norm h0 b /\ live h1 c /\ isMultiplication h0 h1 a b c
+	  /\ eval h1 c (2*norm_length-1) = eval h0 a norm_length * eval h0 b norm_length
+	  /\ maxValue h1 c (2*norm_length-1) <= norm_length * pow2 53))
+
+#reset-options "--z3timeout 5 --initial_fuel 0 --max_fuel 0"
+
+let isDegreeReduced (h0:mem) (h1:mem) (b:bigint) =
+  live h0 b /\ live h1 b /\ length b >= 2*norm_length-1
+  /\ v (get h1 b 0) = v (get h0 b 0) + 5 * v (get h0 b 5)
+  /\ v (get h1 b 1) = v (get h0 b 1) + 5 * v (get h0 b 6)
+  /\ v (get h1 b 2) = v (get h0 b 2) + 5 * v (get h0 b 7)
+  /\ v (get h1 b 3) = v (get h0 b 3) + 5 * v (get h0 b 8)
+
+let satisfiesModuloConstraints (h:heap) (b:bigint) : GTot Type0 =
+  live h b /\ length b >= 2*norm_length-1
+  /\ maxValue h b (2*norm_length-1) * 6 < pow2 63
+
+val lemma_freduce_degree_0:
+  h:mem ->
+  b:bigint ->
+  Lemma (requires (satisfiesModuloConstraints h b))
+	(ensures  (satisfiesModuloConstraints h b
+	  /\ 5 * v (get h b 5) < pow2 64 /\ 5 * v (get h b 6) < pow2 64 /\ 5 * v (get h b 7) < pow2 64
+	  /\ 5 * v (get h b 7) < pow2 64 /\ 5 * v (get h b 8) < pow2 64
+	  /\ v (get h b 0) + 5 * v (get h b 5) < pow2 64 /\ v (get h b 1) + 5 * v (get h b 6) < pow2 64
+	  /\ v (get h b 2) + 5 * v (get h b 7) < pow2 64 /\ v (get h b 3) + 5 * v (get h b 8) < pow2 64
+	))
+let lemma_freduce_degree_0 h b =
+  pow2_double_sum 63;
+  maxValue_lemma_aux h b (2*norm_length-1)
+
+
+let bound63 (h:heap) (b:bigint) : GTot Type0 =
+  live h b /\ v (get h b 0) < pow2 63 /\ v (get h b 1) < pow2 63 /\ v (get h b 2) < pow2 63
+  /\ v (get h b 3) < pow2 63 /\ v (get h b 4) < pow2 63
+
+assume val lemma_freduce_degree:
+  h0:mem ->
+  h1:mem ->
+  b:bigint ->
+  Lemma (requires (satisfiesModuloConstraints h0 b /\ isDegreeReduced h0 h1 b))
+	(ensures  (satisfiesModuloConstraints h0 b /\ isDegreeReduced h0 h1 b
+	  /\ bound63 h1 b
+	  /\ eval h1 b norm_length % reveal prime = eval h0 b (2*norm_length-1) % reveal prime))
+
+#reset-options "--z3timeout 20 --initial_fuel 0 --max_fuel 0"
+
+let isCarried (h0:mem) (h1:mem) (b:bigint) : GTot Type0 =
+  live h0 b /\ live h1 b /\ length b >= norm_length+1
+  /\ (
+      let b0 = v (get h0 b 0) in
+      let b1 = v (get h0 b 1) in
+      let b2 = v (get h0 b 2) in
+      let b3 = v (get h0 b 3) in
+      let b4 = v (get h0 b 4) in
+      let r0  = b0 / pow2 26 in
+      let r1  = (b1 + r0) / pow2 26 in
+      let r2  = (b2 + r1) / pow2 26 in
+      let r3  = (b3 + r2) / pow2 26 in
+      v (get h1 b 5) = (b4 + r3) / pow2 26
+      /\ v (get h1 b 0) = b0 % pow2 26
+      /\ v (get h1 b 1) = (b1 + r0)  % pow2 26
+      /\ v (get h1 b 2) = (b2 + r1)  % pow2 26
+      /\ v (get h1 b 3) = (b3 + r2)  % pow2 26
+      /\ v (get h1 b 4) = (b4 + r3)  % pow2 26
+    )
+
+#reset-options "--z3timeout 20 --initial_fuel 0 --max_fuel 0"
+
+
+let u633 = x:U64.t{v x < pow2 63}
+
+#reset-options "--z3timeout 5 --initial_fuel 0 --max_fuel 0"
+
+
+let isCarried_
+  (h1:mem)
+  (b0:U64.t) (b1:U64.t) (b2:U64.t) (b3:U64.t) (b4:U64.t)
+  (b:bigint) : GTot Type0 =
+  live h1 b /\ length b >= norm_length+1
+  /\ (
+      let r0  = v b0 / pow2 26 in
+      let r1  = (v b1 + r0) / pow2 26 in
+      let r2  = (v b2 + r1) / pow2 26 in
+      let r3  = (v b3 + r2) / pow2 26 in
+      v (get h1 b 5) = (v b4 + r3) / pow2 26
+      /\ v (get h1 b 0) = v b0 % pow2 26
+      /\ v (get h1 b 1) = (v b1 + r0)  % pow2 26
+      /\ v (get h1 b 2) = (v b2 + r1)  % pow2 26
+      /\ v (get h1 b 3) = (v b3 + r2)  % pow2 26
+      /\ v (get h1 b 4) = (v b4 + r3)  % pow2 26
+    )
+
+
+let carried_1 (h:mem) (b:bigint) : GTot Type0 =
+  live h b /\ length b >= norm_length+1
+  /\ v (get h b 0) < pow2 26
+  /\ v (get h b 1) < pow2 26
+  /\ v (get h b 2) < pow2 26
+  /\ v (get h b 3) < pow2 26
+  /\ v (get h b 4) < pow2 26
+  /\ v (get h b 5) <= pow2 38
+
+assume val lemma_carry_1:
+  h0:mem -> h1:mem ->
+  b:bigint{length b >= norm_length+1} ->
+  Lemma (requires (bound63 h0 b /\ isCarried h0 h1 b))
+	(ensures  (bound63 h0 b /\ isCarried h0 h1 b
+	  /\ eval h1 b (norm_length+1) = eval h0 b norm_length /\ carried_1 h1 b))
+
+
+let carried_2 (h:mem) (b:bigint) : GTot Type0 =
+  live h b /\ length b >= norm_length+1
+  /\ v (get h b 0) < pow2 42
+  /\ v (get h b 1) < pow2 26
+  /\ v (get h b 2) < pow2 26
+  /\ v (get h b 3) < pow2 26
+  /\ v (get h b 4) < pow2 26
+
+
+let carried_3 (h:mem) (b:bigint) : GTot Type0 =
+  norm h b /\ length b >= norm_length+1
+  /\ v (get h b 5) <= 1
+  /\ (v (get h b 5) = 1
+    ==> (v (get h b 1) < pow2 18 /\ v (get h b 2) < pow2 18  /\ v (get h b 3) < pow2 18
+	/\ v (get h b 4) < pow2 18))
+
+assume val lemma_carry_2:
+  h0:mem -> h1:mem ->
+  b:bigint{length b >= norm_length+1} ->
+  Lemma (requires (carried_2 h0 b /\ isCarried h0 h1 b))
+	(ensures  (carried_2 h0 b /\ isCarried h0 h1 b
+	  /\ eval h1 b (norm_length+1) = eval h0 b norm_length
+	  /\ carried_3 h1 b))
+
+let carriedTopBottom (h0:mem) (h1:mem) (b:bigint) : GTot Type0 =
+  live h0 b /\ live h1 b /\ length b >= norm_length+1
+  /\ v (get h1 b 0) = v (get h0 b 0) + 5 * v (get h0 b 5)
+  /\ v (get h1 b 1) = v (get h0 b 1)
+  /\ v (get h1 b 2) = v (get h0 b 2)
+  /\ v (get h1 b 3) = v (get h0 b 3)
+  /\ v (get h1 b 4) = v (get h0 b 4)
+
+
+assume val lemma_carry_top_1:
+  h0:mem -> h1:mem ->
+  b:bigint ->
+  Lemma (requires (carried_1 h0 b /\ carriedTopBottom h0 h1 b))
+	(ensures  (carried_1 h0 b /\ carriedTopBottom h0 h1 b
+	  /\ carried_2 h1 b
+	  /\ eval h1 b norm_length % reveal prime = eval h0 b (norm_length+1) % reveal prime))
+
+
+let carried_4 (h:mem) (b:bigint) : GTot Type0 =
+  live h b /\ v (get h b 0) < pow2 26 + 5
+  /\ v (get h b 1) < pow2 26
+  /\ (v (get h b 0) >= pow2 26 ==> v (get h b 1) < pow2 18)
+  /\ v (get h b 2) < pow2 26
+  /\ v (get h b 3) < pow2 26
+  /\ v (get h b 4) < pow2 26
+
+
+assume val lemma_carry_top_2:
+  h0:mem -> h1:mem ->
+  b:bigint ->
+  Lemma (requires (norm h0 b /\ length b >= norm_length + 1
+		  /\ v (get h0 b 5) <= 1 /\ carriedTopBottom h0 h1 b))
+	(ensures  (norm h0 b /\ length b >= norm_length + 1
+	  /\ v (get h0 b 5) <= 1 /\ carriedTopBottom h0 h1 b
+	  /\ eval h1 b norm_length % reveal prime = eval h0 b (norm_length+1) % reveal prime
+	  /\ carried_4 h1 b))
+
+
+let isCarried01 (h0:mem) (h1:mem) (b:bigint) =
+  live h0 b /\ live h1 b
+  /\ v (get h1 b 0) = v (get h0 b 0) % pow2 26
+  /\ v (get h1 b 1) = v (get h0 b 1) + (v (get h0 b 0) / pow2 26)
+  /\ v (get h1 b 2) = v (get h0 b 2)
+  /\ v (get h1 b 3) = v (get h0 b 3)
+  /\ v (get h1 b 4) = v (get h0 b 4)
+
+assume val lemma_carry_0_to_1:
+  h0:mem -> h1:mem ->
+  b:bigint ->
+  Lemma (requires (carried_4 h0 b /\ isCarried01 h0 h1 b))
+	(ensures  (carried_4 h0 b /\ isCarried01 h0 h1 b
+	  /\ norm h1 b /\ eval h1 b norm_length = eval h0 b norm_length))
